LeanCats/Lemmas.lean
@@ -1,4 +1,5 @@
 import LeanCats.HerdingCats
+import Mathlib.Tactic.Linarith.Frontend
 
 open Primitives
 
@@ -83,7 +84,7 @@ lemma tc_N_succ_steps_includes_N_succ
       }
 
 -- This is the tail definition of the TransGen.
-lemma tc_step_trans
+lemma tc_step__base_trans
   {a b c: Event}
   (input : List Event)
   (r : Event -> Event -> Prop)
@@ -138,6 +139,42 @@ lemma tc_step_trans'
       aesop
     }
 
+lemma imm_in_tc_base
+  {r}
+  [DecidableRel r]
+  {a b: Event}
+  (input : List Event)
+  {tc : List (Event × Event)}
+  (h₁ : (a, b) ∈ tc_base r input) :
+  b ∈ input :=
+  by
+    induction tc with
+    | nil => {
+      aesop
+    }
+    | cons head tail tail_ih => {
+      aesop
+    }
+
+lemma imm_in_tc_step_N
+  {n}
+  {r}
+  [DecidableRel r]
+  {a b: Event}
+  (input : List Event)
+  {tc : List (Event × Event)}
+  (h₁ : (a, b) ∈ tc_step_N n input (tc_base r input)) :
+  b ∈ input :=
+  by
+    induction n with
+    | zero => {
+      aesop
+    }
+    | succ n' ih => {
+      apply ih
+      sorry
+    }
+
 lemma tc_step_N_trans
   {n : Nat}
   {a b c: Event}
@@ -159,6 +196,83 @@ lemma tc_step_N_trans
     exact hc
     exact h₁
     exact h₂
+
+lemma tc_base_in_tc_step_N
+  {r}
+  [DecidableRel r]
+  (n : Nat)
+  (input : List Event) :
+  tc_base r input ⊆ tc_step_N n input (tc_base r input) :=
+  by
+    induction n with
+    | zero => {
+      simp
+    }
+    | succ n' ih => {
+      unfold tc_step_N
+      rw [tc_step_N_swap]
+      aesop
+    }
+
+lemma tc_step_N_base_trans
+  (n : Nat)
+  {a b c: Event}
+  (input : List Event)
+  (ha : a ∈ input)
+  (hb : b ∈ input)
+  (hc : c ∈ input)
+  (r : Event -> Event -> Prop)
+  [DecidableRel r]
+  (h₁ : (a, b) ∈ tc_step_N n input (tc_base r input))
+  (h₂ : (b, c) ∈ tc_base r input) :
+  (a, c) ∈ tc_step_N (n+1) input (tc_base r input) :=
+  by
+    unfold tc_step_N
+    rw [tc_step_N_swap]
+    apply tc_step_trans'
+    exact ha
+    exact hb
+    exact hc
+    exact h₁
+    apply tc_base_in_tc_step_N
+    exact h₂
+
+lemma tc_step_N_base_trans'
+  (n : Nat)
+  (a b c: Event)
+  (input : List Event)
+  (r : Event -> Event -> Prop)
+  [DecidableRel r]
+  (h₁ : (a, b) ∈ tc_step_N n input (tc_base r input))
+  (h₂ : (b, c) ∈ tc_base r input) :
+  (a, c) ∈ tc_step_N (n+1) input (tc_base r input) :=
+  by
+    unfold tc_step_N
+    rw [tc_step_N_swap]
+    sorry
+
+-- lemma tc_comp_trans
+--   {n : Nat}
+--   {a b c: Event}
+--   (input : List Event)
+--   {ha : a ∈ input}
+--   {hb : b ∈ input}
+--   {hc : c ∈ input}
+--   (r : Event -> Event -> Prop)
+--   [DecidableRel r]
+--   (h₁ : (a, b) ∈ comp_tc input r)
+--   (h₂ : (b, c) ∈ comp_tc input r) :
+--   (a, c) ∈ comp_tc input r :=
+--   by
+--     unfold comp_tc at *
+--     rw [tc_step_N_swap]
+--     apply tc_step_trans'
+--     exact ha
+--     exact hb
+--     exact hc
+--     exact h₁
+--     apply tc_base_in_tc_step_N
+--     exact h₂
 
 lemma tc_N_steps_in_tc_N_succ'
   {a b : Event}
@@ -223,16 +337,16 @@ lemma TransGen_tc_step
     aesop
 
 lemma tc_N_steps_is_tc
-  {a b: Event}
-  (n : Nat)
+  (a b: Event)
+  {n : Nat}
   (r : Event -> Event -> Prop)
   [DecidableRel r]
   (input : List Event)
-  {ha : a ∈ input}
-  {hb : b ∈ input}
+  (ha : a ∈ input)
+  (hb : b ∈ input)
   {tc : List (Event × Event)}
-  (htrans : ∀ a b, (a, b) ∈ tc -> Relation.TransGen r a b)
-  : (a, b) ∈ tc_step_N n input tc -> Relation.TransGen r a b := by
+  (htrans : ∀ a b, (a, b) ∈ tc -> Relation.TransGen (fun x y => r x y ∧ x ∈ input ∧ y ∈ input) a b)
+  : (a, b) ∈ tc_step_N n input tc -> Relation.TransGen (fun x y => r x y ∧ x ∈ input ∧ y ∈ input) a b := by
     intro h'
     induction n generalizing tc with
     | zero => {
@@ -252,24 +366,21 @@ lemma comp_tc_towards_tc
   a ∈ input
   -> b ∈ input
   -> (a, b) ∈ comp_tc input r
-  -> Relation.TransGen r a b := by
+  -> Relation.TransGen (fun x y => r x y ∧ x ∈ input ∧ y ∈ input) a b := by
     intro ha hb
     unfold comp_tc
     intro h
-    apply tc_N_steps_is_tc
-    exact ha
-    exact hb
-    have hbase : ∀ (a b : Event), (a, b) ∈ (tc_base r input) → Relation.TransGen r a b :=
+    apply tc_N_steps_is_tc a b r input ha hb
+
+    have hbase : (a, b) ∈ (tc_base r input) → Relation.TransGen (fun x y => r x y ∧ x ∈ input ∧ y ∈ input) a b :=
     by
-      intro a b
       intro h'
       simp at h'
       apply And.right at h'
       apply Relation.TransGen.single
-      exact h'
+      aesop
 
-    exact hbase
-    exact h
+    sorry
 
 lemma tc_base_in_product
   (r : Event -> Event -> Prop)
@@ -305,45 +416,12 @@ lemma tc_step_N_in_product
       aesop
     }
 
-lemma tc_base_in_tc_step_N
-  {r}
-  [DecidableRel r]
-  (n : Nat)
-  (input : List Event) :
-  tc_base r input ⊆ tc_step_N n input (tc_base r input) :=
-  by
-    induction n with
-    | zero => {
-      simp
-    }
-    | succ n' ih => {
-      unfold tc_step_N
-      rw [tc_step_N_swap]
-      aesop
-    }
-
--- Every pairs are connected (transitive)
--- This states that the product contains all the possible results.
--- lemma tc_comp_upper_bound
---   {a b : Event}
---   (r : Event -> Event -> Prop)
---   [DecidableRel r]
---   (input : List Event)
---   (ha : a ∈ input)
---   (hb : b ∈ input) :
---   (comp_tc input r) ⊆ input.product input :=
---   by
---     intro p hcomp
---     unfold comp_tc at hcomp
---     apply (tc_step_N_in_product r (input.length * input.length) input)
---     exact hcomp
-
-
 -- We want to calcualte the maximum or minimum pairs we can add for each round.
 -- We need to specify the mimimum rounds that can make sure we can find all the pairs.
 -- Suppose we only filter out one pair in each round, then we need at least (tc.product tc).length to get all the pairs.
 -- 1. First we need to make sure that the input.product input is the upper bound, we can't find any more pair that is out of this bound.
 -- 2. We split the tc_comp, for a b in it, we can find TransGen (a, b) ∧ TransGen (b, c) in previous round, for a b we can need to find (a, e) and (e, b) ...
+-- 3. We find the longest path, use tc_step_N to represent it then because all other steps are smaller than it, it's the subset of setp_N max_len
 
 -- Every pairs are connected (transitive)
 -- This states that the product contains all the possible results.
@@ -357,50 +435,203 @@ lemma tc_comp_upper_bound
     apply tc_step_N_in_product
     aesop
 
+lemma tc_base_is_r
+  {a b: Event}
+  (r : Event -> Event -> Prop)
+  [DecidableRel r]
+  (input : List Event)
+  (ha : a ∈ input)
+  (hb : b ∈ input) :
+  r a b ↔ (a, b) ∈ tc_base r input :=
+  by
+    apply Iff.intro
+    {
+      simp_all
+    }
+    {
+      simp_all
+    }
+
+-- Try to find the event from decoupling the TransGen a b, to say all the intermediate val we say c, is in input.
+-- where c is ∃c, a, c ∨ c, d ...
+-- TransGen r a z if and only if there exists a sequence a r b r ... r z of length at least 1 connecting a to z.
+lemma tc_comp_N_monotonic
+  {i k : Nat}
+  {tc : List (Event × Event)}
+  (r : Event -> Event -> Prop)
+  [DecidableRel r]
+  (input : List Event) :
+  tc_step_N i input tc ⊆ tc_step_N (i+k) input tc :=
+  by
+    rw [tc_step_N_add]
+    induction k with
+    | zero => {
+      simp
+    }
+    | succ n' ih => {
+      rw [tc_step_N]
+      rw [tc_step_N_swap]
+      aesop
+    }
+
+lemma tc_comp_includes_all
+
+lemma tc_comp_includes_all
+  {a b : Event}
+  {r}
+  {n}
+  [DecidableRel r]
+  {input : List Event}
+  (htrans : Relation.TransGen (fun x y => r x y ∧ x ∈ input ∧ y ∈ input) a b) :
+  (a, b) ∈ comp_tc input r -> (a, b) ∈ tc_step_N n input (tc_base r input) :=
+  by
+    intro h
+    aesop
+
 -- We need to prove, after some iterations the (a, b) won't be changed
 -- The computation is limited by input, so the input.product input is what we can calcuate at most.
 -- a ∧ b ∈ input means the all possible results are combinations of (a, b)
 lemma tc_towards_comp_tc
-  {a c : Event}
-  (r : Event -> Event -> Prop)
+  {r : Event -> Event -> Prop}
+  {a b : Event}
   [DecidableRel r]
   (input : List Event) :
   a ∈ input
-  -> c ∈ input
-  -> Relation.TransGen r a c
-  -> (a, c) ∈ comp_tc input r :=
+  -> b ∈ input
+  -> Relation.TransGen (fun x y => r x y ∧ x ∈ input ∧ y ∈ input) a b
+  -> (a, b) ∈ comp_tc input r :=
   by
     intro ha
     intro hb
     intro htrans
     unfold comp_tc
-    induction htrans with
-    | single hrel => {
-      rename_i b
-      apply tc_base_in_tc_step_N
-      simp
-      apply And.intro
-      apply And.intro
-      exact ha
-      exact hb
-      exact hrel
+    unfold tc_step_N
+
+    split
+    {
+      aesop
     }
-    | tail htrans hrel ih => {
-      sorry
-      -- rename_i b
-      -- rename_i c
-      -- induction input with
-      -- | nil => {
-      --   simp_all
-      -- }
-      -- | cons head tail tail_ih => {
-      --   apply tc_step_N_trans
-      --   exact ha
-      --   exact hb
-      --   exact hb
-      -- }
-      -- _
+    {
+      rename_i heq
+      rename_i n'
+      rename_i n
+      rw [<-tc_step_N]
+      induction htrans with
+      | single hrel => {
+        apply tc_base_in_tc_step_N
+        aesop
+      }
+      | tail htrans hrel ih => {
+        rename_i c'
+        rename_i b'
+
+        apply tc_step_N_base_trans' n' a b' c'
+        {
+          induction n with
+          | zero => {
+            apply tc_comp_includes_all
+            {
+              exact htrans
+            }
+            {
+              aesop
+            }
+          }
+          | succ n'' ih => {
+            exact ih
+          }
+        }
+        {
+          aesop
+        }
+      }
     }
+
+#check tc_step_N_trans
+    -- apply tc_step_N_base_trans input.length input ha hb hc r
+
+    -- induction htrans with
+    -- | single hrel => {
+    --   rename_i b
+    --   apply tc_base_in_tc_step_N
+    --   simp
+    --   apply And.intro
+    --   apply And.intro
+    --   exact ha
+    --   exact hb
+    --   exact hrel
+    -- }
+    -- | tail htrans hrel ih => {
+    --   rename_i c'
+    --   rename_i b'
+    --   -- apply tc_step_N_base_trans input r
+    --   -- have htransab' : Relation.TransGen r a b' :=
+    --   -- by
+    --   --   apply Relation.TransGen.tail
+    --   --   exact htrans
+    --   --   exact hrel
+    --   -- apply tc_towards_comp_tc at htransab'
+    --   -- rename_i htransab''
+    -- }
+
+-- For any events a, b we can always find a path.
+
+-- lemma tc_towards_comp_tc'
+--   {a b : Event}
+--   [DecidableRel r]
+--   (input : List Event) :
+--   a ∈ input
+--   -> b ∈ input
+--   -> Relation.TransGen r a b
+--   -> (a, b) ∈ comp_tc' input r :=
+--   by
+--     intro ha
+--     intro hb
+--     intro htrans
+--     unfold comp_tc'
+--     induction htrans with
+--     | single hrel => {
+--
+--     }
+--     | tail htrans rel ih => {
+--       unfold tc_step_N'
+--       split
+--       {
+--
+--       }
+--       {
+--         rename_i len
+--         rename_i n
+--         rename_i n'
+--         induction n
+--       }
+--     }
+
+lemma is_transitive_transGen
+  {a b : Event}
+  (r : Event -> Event -> Prop)
+  [DecidableRel r]
+  (tc : List (Event × Event))
+  (h : ∀p ∈ tc, Relation.TransGen r p.1 p.2)
+  : is_transitive tc (a, b) -> Relation.TransGen r a b :=
+  by
+    simp
+    intro e
+    intro h₁
+    intro h₂
+    have hae : Relation.TransGen r a e :=
+    by
+      apply h (a, e)
+      exact h₁
+
+    have heb : Relation.TransGen r e b :=
+    by
+      apply h (e, b)
+      exact h₂
+
+    apply Relation.TransGen.trans hae heb
+
+-- If the pair is not in the (all input), then it's not a transGen.
 
 theorem tc_comp_is_tc
   {a b : Event}
@@ -409,7 +640,7 @@ theorem tc_comp_is_tc
   (input : List Event)
   (ha : a ∈ input)
   (hb : b ∈ input) :
-  Relation.TransGen r a b <-> (a, b) ∈ comp_tc input r :=
+  Relation.TransGen (fun x y => r x y ∧ x ∈ input ∧ y ∈ input) a b <-> (a, b) ∈ comp_tc input r :=
   by
     apply Iff.intro
     {
@@ -421,9 +652,7 @@ theorem tc_comp_is_tc
       {
         exact hb
       }
-      {
-        exact htrans
-      }
+      sorry
     }
     {
       intro hcomp
@@ -439,13 +668,110 @@ theorem tc_comp_is_tc
       }
     }
 
+-- tc_step_N number of elements can't larger than the (all input).
+-- lemma test_length_lim : tc_step_N := sorry
+
+-- lemma tc_step'_N_swap
+--   (n : Nat)
+--   (input : List Event)
+--   (tc : List (Event × Event)) :
+--   tc_step_N' n input (tc_step input tc) = tc_step input (tc_step_N n input tc) :=
+--   by
+--     induction n generalizing tc with
+--     | zero => {
+--       aesop
+--     }
+--     | succ n' h' => {
+--       rw [tc_step_N]
+--       rw [tc_step_N]
+--       rw [h' (tc_step input tc)]
+--     }
+
+@[simp] def tc_step_N_NoDup
+  (n : Nat)
+  (bound : List (Event × Event))
+  (tc : List (Event × Event))
+  (htc : tc.Nodup)
+  (hb : bound.Nodup)
+  : tc_step_N' n bound tc |>.Nodup :=
+  by
+    induction n with
+    | zero => {
+      simp
+      exact htc
+    }
+    | succ n' ih => {
+      unfold tc_step_N'
+      sorry
+    }
+
+-- @[simp] lemma tc_base_NoDup
+--   (r : Event -> Event -> Prop)
+--   [DecidableRel r]
+--   (input : List Event)
+--   (hinput : input.Nodup)
+--   : tc_base r input |>.Nodup :=
+--   by
+--     simp [List.Nodup]
+--     have prod_nodup : input.product input |>.Nodup :=
+--     by
+--       simp [List.Nodup] at *
+--       induction input with
+--       | nil => {
+--         simp [List.product]
+--       }
+--       | cons head tail ih => {
+--
+--       }
+
+@[simp] def tc_step_NoDup
+  (n : Nat)
+  (bound : List (Event × Event))
+  (tc : List (Event × Event))
+  (htc : tc.Nodup)
+  (hb : bound.Nodup)
+  : tc_step' bound tc |>.Nodup :=
+  by
+    induction n with
+    | zero => {
+      simp
+
+    }
+    | succ n' ih => {
+      unfold tc_step_N'
+      sorry
+    }
+
 instance
   {a b : Event}
   {r : Event -> Event -> Prop}
   [DecidableRel r]
   (input : List Event)
   (ha : a ∈ input)
-  (hb : b ∈ input) : Decidable (Relation.TransGen r a b) :=
+  (hb : b ∈ input) : Decidable (Relation.TransGen (fun x y => r x y ∧ x ∈ input ∧ y ∈ input) a b) :=
   by
     rw [tc_comp_is_tc r input ha hb]
     apply List.instDecidableMemOfLawfulBEq
+
+-- Iterative application of tc_step
+def S_iter (k : Nat) (elems : List Event) (initial_tc : List (Event × Event)) : List (Event × Event) :=
+  match k with
+  | 0 => initial_tc
+  | Nat.succ k_prev => tc_step elems (S_iter k_prev elems initial_tc)
+
+-- Prove that tc_step_N is equivalent to S_iter
+lemma tc_step_N_eq_S_iter (n : Nat) (elems : List Event) (initial_tc : List (Event × Event)) :
+    tc_step_N n elems initial_tc = S_iter n elems initial_tc := by
+  induction n with
+  | zero => simp [tc_step_N, S_iter]
+  | succ n' ih =>
+    rw [tc_step_N, S_iter]
+    rw [<-ih]
+    rw [tc_step_N_swap]
+
+def S (k : Nat) (elems : List Event) (r : Event → Event → Prop) [DecidableRel r] : List (Event × Event) :=
+  S_iter k elems (tc_base r elems)
+
+lemma comp_tc_eq_S_len (elems : List Event) (r : Event → Event → Prop) [DecidableRel r] :
+    comp_tc elems r = S elems.length elems r := by
+  simp [comp_tc, S, tc_step_N_eq_S_iter]
